Lp2lc/Active/TODO.md
@@ -1,0 +1,6 @@
+- Ty.Denotation should be gone, term in PHOAS is already describing denotational syntax
+- Semantics should have better names and definition to handle extrinsic typing
+- merge Ty and Tm into inductive AST
+- make it parametrically extendable
+- extend to System F and FSub
+
